lib/coq/CFML_C.v
@@ -1,0 +1,556 @@
+Set Implicit Arguments.
+
+From CFML Require Import Semantics LibSepFmap.
+Import LibListNotation.
+
+Add Rec LoadPath "../../../CompCert" as compcert.
+Add Rec LoadPath "../../../CompCert/flocq" as Flocq.
+From compcert Require Import Coqlib Maps Integers Floats Values Errors.
+
+(** * Formalizing CFML's fragment resulting from the parsing of C programs *)
+
+(* We compile CFML's language down to CLight.
+   In practice, we only compile a subset of CFML, although we do not reflect this subset statically.
+   The subset corresponds to C programs parsed into CFML. It can be roughly described by the following BNF,
+   obtained after a preprocessing phase (to be written as of now):
+
+   (program)  p ::= list f
+   (function) f ::= { name ; rettype: τ; params: list (var * τ); vars: σ; temps: σ; body: t }
+   (env_var)  σ ::=
+   (prims)    ρ ::= free (heap x) | alloc e
+   (fun)      φ ::= name f | ρ
+   (terms)    t ::= | e
+
+                    | let const x = φ t* in t
+                    | let const x = e in t
+                    | let stack x = undef in t
+                    | let heap  p = var const x in t
+
+                    | let _       = t in t   *
+                    | stack x := e
+                    | heap  x := e
+
+                    | let _       = t in t
+                    | if e then t else t
+                    | while e do t
+
+   (expr)     e ::= v | var flag x | get x | e + e | e < e
+   (values)   v ::= undef | i | f | loc i
+   (types)    τ ::= long | double | ref τ
+
+Note: get x   == trm_apps (val_prim val_get) [x]
+Note: x ::= v == trm_apps (val_prim val_set) [x;v]
+
+ *)
+
+
+
+(** CFML types *)
+
+(* Definition program := list toplevel_fundef
+   fundef := {name, rettype, list (var*type), trm}
+
+   Clight.program -> main : "main"
+
+   Definition tr_program (p : program) : mon Clight.program
+
+   Definition gather_vars (t : trm_r) : list (ident*type)
+   Definition gather_temps (t : trm_r) : list (ident*type)
+
+   Definition tr_trm_stmt (E : env_var) (t: trm_r) : mon Clight.statement
+   Definition tr_trm_expr (E : env_var) (t: trm_r) : mon Clight.expr
+
+   Definiton env_var := Ptree.t var_descr
+
+   Inductive var_descr :=
+    | var_stack
+    | var_heap
+    | var_const
+
+
+   Definition trm_get_var_heap_inv (E : env_var) (t : trm) :
+                                       option (ident*type) :=
+      match t with
+      | trm_app trm_get (trm_var x :: nil) =>
+                       match Ptree.get E x with
+                       | Some (var_heap) => Some x
+                       | _ => None
+      | _ => None
+
+ *)
+
+Unset Elimination Schemes.
+
+Section CFML_TYPES.
+
+Inductive type : Type :=
+| type_long : type
+| type_double : type
+| type_ref : type -> type.
+
+Variant var_descr : Type :=
+  | stack : var_descr
+  | heap : var_descr
+  | const : var_descr.
+
+Global Instance Inhab_var_descr_type : Inhab (var_descr * type).
+Proof using. apply (Inhab_of_val (stack,type_long)). Qed.
+
+
+Definition var' : Type := var * (option AST.ident).
+Coercion var_to_var' (x : var) : var' := (x, None).
+
+
+Definition var'_eq (x y : var') : bool :=
+  match x, y with
+  | (xv, Some xi), (yv, Some yi) =>
+      if (eq_var_dec xv yv) then (Pos.eqb xi yi) else false
+  | _, _ => false
+  end.
+
+
+Definition get_ident (x : var') : res AST.ident :=
+  match x with
+  | (v, Some i) => OK i
+  | (v, None) => Error (msg "get_ident: no set ident" ++ msg v)
+  end.
+
+(* Redefiniton of LibSepBind.bind to be typed, and with var descr *)
+Inductive binding : Type :=
+| binding_anon : binding
+| binding_var : var' -> type -> var_descr -> binding.
+
+Definition numtype := type.
+
+Variant prim : Type :=
+  | val_ptr_add : prim
+  | val_add : numtype -> prim
+  (* | val_cast : numtype -> numtype -> prim
+      (en pratique, juste besoin de (val_cast type_long type_double))*)
+  | val_lt : numtype -> prim
+  | val_ref : prim
+  | val_get : prim
+  | val_set : prim
+  | val_free : prim
+  | val_alloc : prim
+  | val_dealloc : prim.
+
+
+Definition is_binop (op : prim) : bool :=
+  match op with
+  | val_add _
+  | val_lt _
+    => true
+  | _ => false
+  end.
+
+Inductive val : Type :=
+| val_uninitialized : val
+| val_unit : val
+| val_int : int -> val
+| val_loc : loc -> val
+| val_prim : prim -> val
+
+with trm : Type :=
+| trm_val : val -> trm
+| trm_var : var' -> trm
+| trm_apps : trm -> list trm -> trm
+| trm_let : binding -> trm -> trm -> trm
+| trm_while : trm -> trm -> trm
+| trm_ite : trm -> trm -> trm -> trm.
+
+
+Definition trm_seq (t1 t2 : trm) : trm :=
+  trm_let binding_anon t1 t2.
+
+Definition env_var := PTree.t (var_descr*type).
+
+Definition env_var_join (E1 E2 : env_var) : env_var :=
+  PTree.fold (fun t k elt => PTree.set k elt t) E1 E2.
+
+(* Definition env_var := fmap var (var_descr*type). *)
+
+Record fundef : Type :=
+  mkfundef {
+      name: var';
+      rettype: type;
+      params: list (var' * type);
+      vars: env_var;
+      temps: env_var;
+      body: trm
+  }.
+
+
+(* The choice is made here that function paramenters are temporaries (const in cfml),
+   do not reside in memory, and thus their address cannot be referenced. This choice
+   corresponds to the semantic [function_entry2] of Clight. (read Clight.v:547,713)*)
+
+Definition program := list fundef.
+
+End CFML_TYPES.
+
+Coercion val_prim : prim >-> val.
+Coercion val_loc : loc >-> val.
+Coercion trm_var : var' >-> trm.
+Coercion trm_val : val >-> trm.
+
+Definition state : Type := fmap loc val.
+
+Implicit Types v : val.
+Implicit Type l : loc.
+Implicit Types t : trm.
+Implicit Types s : state.
+Implicit Types op : prim.
+Implicit Types P : state -> trm -> Prop.
+
+Inductive combiner :=
+  | combiner_nil : trm -> trm -> combiner
+  | combiner_cons : combiner -> trm -> combiner.
+
+Coercion combiner_nil : trm >-> Funclass.
+Coercion combiner_cons : combiner >-> Funclass.
+
+Fixpoint combiner_to_trm (c:combiner) : trm :=
+  match c with
+  | combiner_nil t1 t2 => trm_apps t1 (t2::nil)
+  | combiner_cons c1 t2 =>
+      match combiner_to_trm c1 with
+      | trm_apps t1 ts => trm_apps t1 (List.app ts (t2::nil))
+      | t1 => trm_apps t1 (t2::nil)
+      end
+  end.
+
+Coercion combiner_to_trm : combiner >-> trm.
+
+Section Trm_induct.
+
+  Variables (P : trm -> Prop)
+    (Q : list trm -> Prop)
+    (Q1 : Q nil)
+    (Q2 : forall t (l : list trm), P t -> Q l -> Q (t::l))
+    (f : forall (v : val), P v)
+    (f0 : forall (v : var'), P v)
+    (f3 : forall (t : trm), P t -> forall t0 : trm, P t0 -> forall t1 : trm, P t1 -> P (trm_ite t t0 t1))
+    (f4 : forall (b : binding) (t : trm), P t -> forall t0 : trm, P t0 -> P (trm_let b t t0))
+    (f5 : forall (t : trm), P t -> forall (l : list trm), Q l -> P (trm_apps t l))
+    (f6 : forall (t : trm), P t -> forall t0 : trm, P t0 -> P (trm_while t t0)).
+
+  Definition trm_induct_gen := fix F (t : trm) : P t :=
+      let trm_list_induct := fix f (l : list trm) : Q l :=
+          match l as x return Q x with
+          | nil   => Q1
+          | t::l' => Q2 (F t) (f l')
+          end in
+      match t as t0 return (P t0) with
+      | trm_val v => @f v
+      | trm_var v => @f0 v
+      | trm_ite t0 t1 t2 => @f3 t0 (F t0) t1 (F t1) t2 (F t2)
+      | trm_let b t0 t1 => @f4 b t0 (F t0) t1 (F t1)
+      | trm_apps t0 l => @f5 t0 (F t0) l (trm_list_induct l)
+      | trm_while t0 t1 => @f6 t0 (F t0) t1 (F t1)
+      end.
+
+End Trm_induct.
+
+Lemma trm_ind : forall P : trm -> Prop,
+  (forall v : val, P v) ->
+  (forall v : var', P v) ->
+  (forall t : trm, P t -> forall t0 : trm, P t0 -> forall t1 : trm, P t1 -> P (trm_ite t t0 t1)) ->
+  (forall (b : binding) (t : trm), P t -> forall t0 : trm, P t0 -> P (trm_let b t t0)) ->
+  (forall t : trm, P t -> forall (l : list trm), (forall t, mem t l -> P t) -> P (trm_apps t l)) ->
+  (forall t : trm, P t -> forall t0 : trm, P t0 -> P (trm_while t t0)) ->
+  forall t : trm, P t.
+Proof using.
+  hint mem_map'.
+  intros. gen t. eapply trm_induct_gen with
+    (Q := fun (l : list trm) => forall t, mem t l -> P t); eauto.
+  { introv M. inverts M. }
+  { introv M1 M2 M3. inverts~ M3. }
+Qed.
+
+
+
+  (** ** int * (const) p = malloc ?     ->  w: *p = v;    r: *p     + free(p);
+    cfml   => let p = val_alloc(1) in
+           w=> (set p v)
+           r=> (get p)
+           free=> (free p)
+
+    clight =>
+           decla d'un `type * p` au début, puis
+              Sbuiltin (Some p) malloc [sizeof(int)];
+           w=> Sassign (Ederef (Evar p)) v
+           r=> Ederef (Evar p)
+           free=> Sbuiltin None free (Evar p)
+   *)
+
+  (** ** int x;         ->   w:   x = v;    r: x
+    cfml   => let p (décoration : stack allocated) = valloc(1) in
+           ... pareil
+
+    clight => ramener au début de la déclaration de la fonction
+              compile_fun => analyse prog, sort liste des variabels
+           w=> Sassign (Evar x) v
+           r=> Evar x
+   *)
+
+  (** ** tempvar = v;
+        => Sset tempvar v / let tempvar = v
+        => clight : decla d'un `register void *$42;` au début
+                      -> pour tout appel de fonction du coup
+   *)
+
+
+Reserved Notation "t '/' s '-->' P"
+  (at level 40, s at level 30).
+
+Global Instance Inhab_val : Inhab val.
+Proof using. apply (Inhab_of_val val_unit). Qed.
+
+
+Fixpoint subst (y:var') (w:val) (t:trm) : trm :=
+  let aux t :=
+    subst y w t in
+  let aux_no_capture z t :=
+    match z with
+    | binding_anon => aux t
+    | binding_var x _ _ => if (var'_eq x y) then t else aux t
+    end in
+    (* If z = binding_var y then t else aux t in *)
+  let aux_no_captures xs t :=
+    If LibList.mem y xs then t else aux t in
+  match t with
+  | trm_val v => trm_val v
+  | trm_var x => If x = y then trm_val w else t
+  | trm_ite t0 t1 t2 => trm_ite (aux t0) (aux t1) (aux t2)
+  | trm_let z t1 t2 => trm_let z (aux t1) (aux_no_capture z t2)
+  | trm_apps t0 ts => trm_apps (aux t0) (LibListExec.map aux ts)
+  | trm_while t1 t2 => trm_while (aux t1) (aux t2)
+  end.
+
+
+Definition subst1 (z:binding) (v:val) (t:trm) :=
+  match z with
+  | binding_anon => t
+  | binding_var x _ _ => subst x v t
+  end.
+
+(* NOTE: substition-based, will need to bridge the gap with the environment-based one on CLight's side *)
+(* NOTE: missing constructs *)
+Inductive cfml_step : state -> trm -> (state->trm->Prop) -> Prop :=
+| cfml_step_val : forall v s P,
+    P s (trm_val v) ->
+    (trm_val v) / s --> P
+
+| cfml_step_seq : forall v1 t2 s P,
+    P s t2 ->
+    (trm_seq (trm_val v1) t2) / s --> P
+
+| cfml_step_seq_l : forall t1 t2 s P P1,
+    t1 / s --> P1 ->
+    (forall t1' s', P1 s' t1' -> (trm_seq t1' t2) / s' --> P) ->
+    (trm_seq t1 t2) / s --> P
+
+| cfml_step_set : forall s l v P,
+    Fmap.indom s l ->
+    P (Fmap.update s l v) val_unit ->
+    (val_set l v) / s --> P
+
+| cfml_step_let : forall s x t2 v1 P,
+    P s (subst1 x v1 t2) ->
+    (trm_let x v1 t2) / s --> P
+
+| cfml_step_ref : forall v s P,
+      (forall l, ~Fmap.indom s l ->
+            l <> null ->
+            P (Fmap.update s l v) (val_loc l)) ->
+      (exists l, ~Fmap.indom s l /\ l <> null) ->
+       (val_ref v)/ s --> P
+
+| cfml_step_get : forall s l P,
+    Fmap.indom s l ->
+    P s (Fmap.read s l) ->
+    (val_get l) / s --> P
+
+| cfml_step_ite : forall s b t1 t2 P,
+    P s (if (b =? 0) then t2 else t1) ->
+    (trm_ite (val_int b) t1 t2) / s --> P
+
+| cfml_step_free : forall s l P,
+    Fmap.indom s l ->
+    P (Fmap.remove s l) val_unit ->
+    (val_free l) / s --> P
+
+| cfml_step_ptr_add : forall l l' n s P,
+    (l':nat) = (l:nat) + n :> int ->
+    P s (val_loc l') ->
+    (val_ptr_add l (val_int n)) / s --> P
+| cfml_step_add : forall s n1 n2 P,
+    P s (val_int (n1 + n2)) ->
+    ((val_add type_long) (val_int n1) (val_int n2)) / s --> P
+
+| cfml_step_lt : forall s n1 n2 P,
+    P s (if (n1 <? n2) then val_int 1 else val_int 0) ->
+    ((val_lt type_long) (val_int n1) (val_int n2)) / s --> P
+
+| cfml_step_alloc : forall n sa P,
+    (forall l k sb, sb = Fmap.conseq (LibList.make k val_uninitialized) l ->
+               n = nat_to_Z k ->
+               l <> null ->
+               Fmap.disjoint sa sb ->
+               P (sb \+ sa) (val_loc l)) ->
+    (exists l k sb, sb = Fmap.conseq (LibList.make k val_uninitialized) l
+               /\ n = nat_to_Z k
+               /\ l <> null
+               /\ Fmap.disjoint sa sb) ->
+     (val_alloc (val_int n)) / sa --> P
+| cfml_step_dealloc : forall (n:int) s l P,
+    (forall vs sa sb, s = sb \+ sa ->
+                 sb = Fmap.conseq vs l ->
+                 n = LibList.length vs ->
+                 Fmap.disjoint sa sb ->
+                 P sa val_unit) ->
+    (exists vs sa sb, s = sb \+ sa
+                 /\ sb = Fmap.conseq vs l
+                 /\ n = LibList.length vs
+                 /\ Fmap.disjoint sa sb) ->
+    (val_dealloc (val_int n) l) / s --> P
+
+where "t / s --> P" := (cfml_step s t P).
+(* TODO à compléter *)
+
+
+(** * Surface syntax for CFML_C *)
+
+(* Custom Syntax (from SLF) *)
+
+Declare Custom Entry trm.
+(* Import LibListNotation. *)
+
+Declare Scope type_scope.
+
+Notation "'long'" := type_long (at level 0, only parsing) : type_scope.
+Notation "'double'" := type_double (at level 0, only parsing) : type_scope.
+Notation "ty 'ref'" :=
+  (type_ref ty) (at level 0, only parsing) : type_scope.
+
+
+Declare Scope trm_scope.
+
+Notation "<{ e }>" :=
+  e
+  (at level 0, e custom trm at level 99) : trm_scope.
+
+Notation "( x )" :=
+  x
+  (in custom trm, x at level 99) : trm_scope.
+
+Notation "'begin' e 'end'" :=
+  e
+  (in custom trm, e custom trm at level 99, only parsing) : trm_scope.
+
+Notation "{ x }" :=
+  x
+  (in custom trm, x constr) : trm_scope.
+
+Notation "x" := x
+  (in custom trm at level 0,
+   x constr at level 0) : trm_scope.
+
+
+Notation "t1 '(' t2 , .. , tn ')'" :=
+  (trm_apps t1 (@cons trm t2 .. (@cons trm tn nil) .. ))
+    (in custom trm at level 30,
+        t2 custom trm at level 99,
+        tn custom trm at level 99,
+      format "t1 '[   ' '(' t2 ',' .. ',' tn ')' ']'") : trm_scope.
+
+Notation "'if' t0 'then' t1 'else' t2" :=
+  (trm_ite t0 t1 t2)
+  (in custom trm at level 69,
+   t0 custom trm at level 99,
+   t1 custom trm at level 99,
+   t2 custom trm at level 99,
+   left associativity,
+   format "'[v' '[' 'if'  t0  'then'  ']' '/' '['   t1 ']' '/' 'else' '/' '['   t2 ']' ']'") : trm_scope.
+
+Notation "'while' t1 'do' t2 'done'" :=
+  (trm_while t1 t2)
+  (in custom trm at level 0,
+   t1 custom trm at level 99,
+   t2 custom trm at level 99,
+   format "'[v' 'while'  t1  'do'  '/' '['   t2 ']' '/'  'done' ']'")
+   : trm_scope.
+
+Notation "t1 ';' t2" :=
+  (trm_let binding_anon t1 t2)
+  (in custom trm at level 68,
+   t2 custom trm at level 99,
+   right associativity,
+   format "'[v' '[' t1 ']' ';' '/' '[' t2 ']' ']'") : trm_scope.
+
+Notation "'let' '(' x ':' ty '#' desc ')' '=' t1 'in' t2" :=
+  (trm_let (binding_var x ty desc) t1 t2)
+  (in custom trm at level 69,
+      x at level 0,
+      ty at level 0,
+      desc at level 0,
+      t1 custom trm at level 100,
+      t2 custom trm at level 100,
+      right associativity,
+      format "'[v' '[' 'let'  '(' x  ':'  ty '#' desc ')'  '='  t1  'in' ']' '/' '[' t2 ']' ']'") : trm_scope.
+
+Notation "'()'" :=
+  (trm_val val_unit)
+  (in custom trm at level 0) : trm_scope.
+
+Notation "'()'" :=
+  (val_unit)
+  (at level 0) : val_scope.
+
+
+Notation "'ref'" :=
+  (trm_val (val_prim val_ref))
+  (in custom trm at level 0) : trm_scope.
+
+
+Notation "'!' t" :=
+  (val_get t)
+  (in custom trm at level 0,
+      t custom trm at level 1,
+      format "'!' t") : trm_scope.
+
+(* Notation "'free'" := *)
+(*   (trm_val (val_prim val_free)) *)
+(*   (in custom trm at level 0) : trm_scope. *)
+
+Notation "'alloc'" :=
+  (trm_val (val_prim val_alloc))
+  (in custom trm at level 0) : trm_scope.
+
+Notation "t1 ':=' t2" :=
+  (val_set t1 t2)
+  (in custom trm at level 67, format "t1  ':='  t2") : trm_scope.
+
+Notation "t1 + t2" :=
+  ((val_add type_long) t1 t2)
+  (in custom trm at level 58) : trm_scope.
+
+Notation "t1 < t2" :=
+  ((val_lt type_long) t1 t2)
+    (in custom trm at level 60) : trm_scope.
+
+
+Module CFMLSyntax.
+
+  Open Scope type_scope.
+  Open Scope trm_scope.
+  Open Scope val_scope.
+  Open Scope string_scope.
+
+  Coercion string_to_var (x:string) : var := x.
+  Coercion int_to_trm (n:int) : trm := (trm_val (val_int n)).
+
+End CFMLSyntax.
+
+
