lib/coq/Clight_omni.v
@@ -1,0 +1,8 @@
+Add Rec LoadPath "../../../CompCert" as compcert.
+Add Rec LoadPath "../../../CompCert/flocq" as Flocq.
+From compcert Require Coqlib Maps Integers Floats Values AST Ctypes Clight.
+From compcert Require Import Maps Errors SimplExpr.
+
+(* We define an omni-small-step semantics for CLight *)
+
+(* TOOD *)
